---
title: "Post14"
author: "Zachary Palmore"
date: "4/27/2021"
output: pdf_document
---

```{r setup, include=FALSE}
knitr::opts_chunk$set(echo = TRUE)
```


## Question

In Exercises 13 â€“ 16, show that the Taylor series for $f(x)$, as
given in Key Idea 8.8.1, is equal to $f(x)$ by applying Theorem
8.8.1; that is, show $\lim\limits_{n\to\infty} R_n(x)=0$.

In this case, we have $f(x) = e^x$.

## Answer

From 8.8.1, we have 

$$f(x) = e^x \hspace{4pt} and \hspace{4pt} f'(x) = e^x$$

And since;

$$d/dx(e^x) = (e^x)$$
$$|R_n(x)| \le \frac{max|f^{n+1}(z)|}{(n+1)!} |x^{n+1}|$$

$$|R_n(x)| \le \frac{e^z}{(n+1)!} |x^{n+1}|$$
$$\lim\limits_{n\to\infty} \frac{e^z x^{n+1}}{(n+1)!} = 0$$
$$\lim\limits_{n\to\infty} R_n(x) = 0$$
Set to 0 we get;

$$f(x) = \sum\limits_{n=0}^{\infty} \frac{f^{(n)}(c)}{n!} (x-c)^n$$
$$f(x) = \sum\limits_{n=0}^{\infty} \frac{e^0}{n!} (x-0)^n = \sum\limits_{n=0}^{\infty} \frac{x^n}{n!} = e^x$$